Verify Assignment forwarding pass
Had to change implementation from collect, then apply, to iteratively
applying each assignment to the ones after it. This requires the
module to be sorted, but that is easy enough to do and trivially
correct (since sorting is already part of the semantics).

Commits
- WIP module_body_inline proof done - Missing collect_substitutions proof
- WIP Use substitution record everywhere
- WIP Fix definition of module_items_sorted
- WIP Reorganized AssignmentForwarding
- WIP on assignment_forwarding proof - admitted lemmas
- WIP applying a substitution does not invalidate the others
- WIP Completely change approach for assignment forwarding
- WIP Qed (with small assumption) on assignment forwarding
  Need to move sort_module_items_idempotent to VerilogSort

vera/VerilogSemantics.v
@@ -75,11 +75,11 @@ Qed.
 
 Ltac disjoint_saturate :=
   repeat match goal with
-         | [ H : disjoint (_ :: _) _ |- _ ] =>
-	   inv H
-         | [ H : disjoint _ (_ :: _) |- _ ] =>
+         | [ H : disjoint (_ :: ?l1) ?l2 |- _ ] =>
+	   inv H; fold (disjoint l1 l2) in *
+         | [ H : disjoint ?l2 (_ :: ?l1) |- _ ] =>
 	   symmetry in H;
-	   inv H
+	   inv H; fold (disjoint l1 l2) in *
          | [ H : disjoint (_ ++ _) _ |- _ ] =>
            rewrite ! disjoint_app_iff in H;
            decompose record H;
@@ -516,18 +516,25 @@ Module CombinationalOnly.
   Definition Process := Verilog.module_item.
 
   Section Sorted.
-    Equations module_items_sorted : list Verilog.module_item -> Prop :=
-      module_items_sorted [] := True;
-      module_items_sorted (mi :: mis) :=
-        Forall (fun mi' => disjoint (Verilog.module_item_writes mi) (Verilog.module_item_reads mi')) mis
-               /\ module_items_sorted mis
+    Inductive module_items_sorted : list Verilog.module_item -> Prop :=
+      | module_items_sorted_nil : module_items_sorted []
+      | module_items_sorted_cons mi mis :
+        disjoint (Verilog.module_body_writes (mi :: mis)) (Verilog.module_item_reads mi) ->
+	module_items_sorted mis ->
+        module_items_sorted (mi :: mis)
     .
 
     Global Instance dec_module_items_sorted ms : DecProp (module_items_sorted ms).
     Proof.
-      induction ms;
-        simp module_items_sorted;
-        try typeclasses eauto.
+      induction ms.
+      - left. constructor.
+      - destruct
+          (dec (disjoint (Verilog.module_body_writes (a :: ms)) (Verilog.module_item_reads a))),
+	  IHms.
+        + left. constructor; assumption.
+	+ right. inversion 1. crush.
+	+ right. inversion 1. crush.
+	+ right. inversion 1. crush.
     Defined.
   End Sorted.
 
@@ -1222,3 +1229,75 @@ Module Equivalence.
     as equivalent_behaviour_rel.
 
 End Equivalence.
+
+Module ExactEquivalence.
+  Import CombinationalOnly.
+  Export Clean.
+
+  Declare Scope verilog.
+  Local Open Scope verilog.
+
+  Record exact_equivalence (v1 v2 : Verilog.vmodule) : Prop :=
+    MkEquivalentBehaviour {
+      inputs_same : Verilog.module_inputs v1 = Verilog.module_inputs v2;
+      outputs_same : Verilog.module_outputs v1 = Verilog.module_outputs v2;
+      execution_match : forall e, (v1 ⇓ e <-> v2 ⇓ e)
+    }.
+
+  Infix "~~~" := exact_equivalence (at level 20) : verilog.
+
+  Lemma exact_equivalence_sym v1 v2:
+    v1 ~~~ v2 ->
+    v2 ~~~ v1.
+  Proof.
+    intros [? ? execution_match].
+    constructor.
+    - symmetry. assumption.
+    - symmetry. assumption.
+    - symmetry. auto.
+  Qed.
+
+  Lemma exact_equivalence_trans v1 v2 v3:
+    v1 ~~~ v2 -> v2 ~~~ v3 -> v1 ~~~ v3.
+  Proof.
+    intros [] [].
+    constructor.
+    - congruence.
+    - congruence.
+    - etransitivity; eauto.
+  Qed.
+
+  Lemma exact_equivalence_refl v : v ~~~ v.
+  Proof. constructor; reflexivity. Qed.
+
+  Add Parametric Relation :
+    Verilog.vmodule exact_equivalence
+    reflexivity proved by exact_equivalence_refl
+    symmetry proved by exact_equivalence_sym
+    transitivity proved by exact_equivalence_trans
+    as exact_equivalence_rel.
+
+  Global Instance Proper_valid_execution_exact_equivalence :
+    Proper (exact_equivalence ==> eq ==> iff) valid_execution.
+  Proof.
+    repeat intro. subst.
+    destruct H. auto.
+  Qed.
+
+  Import Equivalence.
+
+  Lemma exact_equivalence_equivalent_behaviour v1 v2 :
+    clean_module v1 ->
+    clean_module v2 ->
+    v1 ~~~ v2 ->
+    v1 ~~ v2.
+  Proof.
+    intros Hclean1 Hclean2 [].
+    constructor.
+    - assumption.
+    - assumption.
+    - assumption.
+    - assumption.
+    - auto.
+  Qed.
+End ExactEquivalence.
