vera/AssignmentForwarding/AssignmentForwardingCorrect.v
@@ -1,29 +1,303 @@
 From Stdlib Require Import BinNums.
+From Stdlib Require Import List.
+From Stdlib Require Import ProofIrrelevance.
+From Stdlib Require Import String.
+From Stdlib Require Import Setoid.
 
 From Equations Require Import Equations.
 From ExtLib Require Import Structures.Monads.
 
 From vera Require Import Verilog.
 Import Verilog.
+From vera Require Import VerilogSemantics.
+Import CombinationalOnly.
+Import Facts.
+Import ExactEquivalence.
 From vera Require Import Common.
 From vera Require Import Decidable.
 From vera Require Import Tactics.
 From vera Require Import AssignmentForwarding.AssignmentForwarding.
+From vera Require Import VerilogSort.
 
+Import ListNotations.
 Import EqNotations.
 Import MonadLetNotation.
+Import SigTNotations.
 
 Require Import VerilogSemantics.
 Import CombinationalOnly.
 
-Lemma expr_inline_var_correct {w} regs var (replacement : expression (varType var)) (e : expression w) :
-  regs var = eval_expr regs replacement ->
-  eval_expr regs e = eval_expr regs (expr_inline_var var replacement e).
+Local Open Scope verilog.
+
+Lemma not_in_app_iff A (x : A) l1 l2 : ~ In x (l1 ++ l2) <-> (~ In x l1 /\ ~ In x l2).
 Proof.
-  funelim (expr_inline_var var replacement e);
-    intros; simp expr_inline_var eval_expr;
-    try rewrite <- H by assumption;
-    try rewrite <- H0 by assumption;
-    try rewrite <- H1 by assumption;
-    try reflexivity.
+  split; intros.
+  - split; intro contra; contradict H; apply in_app_iff; crush.
+  - destruct H as [H1 H2]. rewrite in_app_iff. intros []; contradiction.
 Qed.
+
+Ltac unpack_in :=
+  repeat match goal with
+         | [ H : ~ (In _ (_ ++ _)) |- _] => apply not_in_app_iff in H; destruct H
+         | [ H : (In _ (_ ++ _)) |- _] => apply in_app_iff in H; destruct H
+         | [ |- ~ In _ (_ ++ _) ] => apply not_in_app_iff; split
+	 end.
+
+Section Apply.
+  Lemma apply_substitution_expr_no_effect {w} (e : expression w) v r :
+    ~ In v (expr_reads e) ->
+    apply_substitution_expr v r e = e.
+  Proof.
+    funelim (apply_substitution_expr v r e);
+      intros; simp expr_reads apply_substitution_expr in *;
+      unpack_in;
+      try rewrite H by assumption;
+      try rewrite H0 by assumption;
+      try rewrite H1 by assumption;
+      crush.
+  Qed.
+  
+  Lemma apply_substitution_expr_correct {w} v r (e : expression w) regs :
+    eval_expr regs r = regs v ->
+    eval_expr regs (apply_substitution_expr v r e) = eval_expr regs e.
+  Proof.
+    funelim (apply_substitution_expr v r e);
+      intros; simp apply_substitution_expr eval_expr;
+      try rewrite H by assumption;
+      try rewrite H0 by assumption;
+      try rewrite H1 by assumption;
+      try reflexivity.
+  Qed.
+
+  Lemma apply_substitution_module_body_valid v r (body : list module_item) regs :
+    eval_expr regs r = regs v ->
+    ~ In v (module_body_writes body) ->
+    disjoint (module_body_writes body) (expr_reads r) ->
+    exec_module_body regs (apply_substitution_module_body v r body) =
+      exec_module_body regs body.
+  Proof.
+    revert regs.
+    funelim (apply_substitution_module_body v r body); [reflexivity|].
+    clear Heqcall.
+    intros * Heval Hvalid Hreads_preserved.
+    simp module_body_writes module_item_writes statement_writes in *. unpack_in.
+    simp exec_module_body exec_module_item in *.
+    destruct lhs; simp expr_reads exec_statement in *; simpl; try reflexivity; expect 1.
+    disjoint_saturate.
+    rewrite ! apply_substitution_expr_correct by assumption.
+    destruct (eval_expr regs rhs) eqn:E; [|reflexivity].
+    apply H; try assumption; expect 1.
+    rewrite RegisterState.set_reg_get_out by crush.
+    rewrite <- Heval.
+    apply eval_expr_change_regs.
+    apply RegisterState.match_on_set_reg_elim.
+    assumption.
+  Qed.
+End Apply.
+
+Lemma apply_substitution_expr_reads w var v r e :
+  In var (expr_reads (apply_substitution_expr (w:=w) v r e)) ->
+  (In var (expr_reads e) \/ In var (expr_reads r)).
+Proof.
+  induction e;
+    intros; simp expr_reads apply_substitution_expr in *;
+    unpack_in; try rewrite ! in_app_iff; try crush; expect 1.
+  match type of H with context[dec ?P] =>
+    destruct (dec P); crush
+  end.
+Qed.
+
+Lemma apply_substitution_writes v r body :
+  module_body_writes (apply_substitution_module_body v r body) = module_body_writes body.
+Proof.
+  funelim (apply_substitution_module_body v r body);
+    simp module_body_writes module_item_writes statement_writes expr_reads in *;
+    crush.
+Qed.
+
+Lemma disjoint_app_iff A (l1 l2 l3 : list A) :
+  (disjoint l1 l3 /\ disjoint l2 l3) <-> (disjoint (l1 ++ l2) l3).
+Proof.
+  unfold disjoint.
+  setoid_rewrite List.Forall_forall.
+  setoid_rewrite in_app_iff.
+  crush.
+Qed.
+
+Lemma apply_substitution_sorted v r body :
+  ~ In v (module_body_writes body) ->
+  disjoint (module_body_writes body) (expr_reads r) ->
+  module_items_sorted body ->
+  module_items_sorted (apply_substitution_module_body v r body).
+Proof.
+  intros Hno_write Hreads_stable Hsorted.
+  funelim (apply_substitution_module_body v r body);
+    simp module_body_writes module_item_writes statement_writes expr_reads in *;
+    expect 1.
+  clear Heqcall.
+  inv Hsorted. unpack_in. disjoint_saturate.
+  simp module_body_writes module_item_writes statement_writes expr_reads in *.
+  constructor; [|apply H; assumption].
+  simp module_body_writes module_item_writes statement_writes
+       expr_reads module_item_reads statement_reads expr_reads in *.
+  disjoint_saturate.
+  rewrite apply_substitution_writes.
+  unfold disjoint. rewrite List.Forall_forall. setoid_rewrite in_app_iff.
+  intros var Hvar_write Hvar_read.
+  apply apply_substitution_expr_reads in Hvar_read.
+  intuition (contradiction || match goal with
+    [ Hin1 : In var ?l1, Hin2 : In var ?l2, Hdisjoint : disjoint ?l1 ?l2 |- _ ] =>
+      eapply disjoint_l_intro; [ eapply Hdisjoint | eapply Hin1 | eapply Hin2 ]
+    end).
+Qed.
+
+Lemma forward_assignments_body_correct regs body body' :
+  NoDup (module_body_writes body) ->
+  module_items_sorted body ->
+  forward_assignments_body body = inr body' ->
+  exec_module_body regs body' = exec_module_body regs body.
+Proof.
+  intros Hnodup Hsorted Hexec.
+  funelim (forward_assignments_body body);
+    rewrite <- Heqcall in *; clear Heqcall; inv Hexec;
+    try reflexivity; expect 1.
+  monad_inv.
+  simp module_body_writes module_item_writes statement_writes expr_reads in *.
+  inv Hnodup. inv Hsorted.
+  simp
+    module_body_writes module_item_writes statement_writes expr_reads
+    module_body_reads module_item_reads statement_reads expr_reads
+    in *.
+  disjoint_saturate.
+  simp exec_module_body exec_module_item exec_statement.
+  destruct (eval_expr regs rhs) eqn:Heval; simpl; [|reflexivity].
+  specialize (H (RegisterState.set_reg var x regs) l).
+  rewrite H; cycle 1.
+  - rewrite apply_substitution_writes. assumption.
+  - apply apply_substitution_sorted; assumption.
+  - reflexivity.
+  - apply apply_substitution_module_body_valid.
+    + rewrite RegisterState.set_reg_get_in.
+      erewrite eval_expr_change_regs; [eassumption|].
+      apply RegisterState.match_on_set_reg_elim.
+      assumption.
+    + assumption.
+    + assumption.
+Qed.
+
+Lemma module_inputs_same v1 v2 :
+  modVariableDecls v1 = modVariableDecls v2 ->
+  module_inputs v1 = module_inputs v2.
+Proof. unfold module_inputs. crush. Qed.
+
+Lemma module_outputs_same v1 v2 :
+  modVariableDecls v1 = modVariableDecls v2 ->
+  module_outputs v1 = module_outputs v2.
+Proof. unfold module_outputs. crush. Qed.
+
+Lemma initial_state_same v1 v2 regs :
+  modVariableDecls v1 = modVariableDecls v2 ->
+  mk_initial_state v1 regs = mk_initial_state v2 regs.
+Proof.
+  unfold mk_initial_state.
+  intros.
+  erewrite module_inputs_same by eassumption.
+  reflexivity.
+Qed.
+
+Lemma sort_module_items_idempotent inputs body :
+  module_items_sorted body ->
+  sort_module_items inputs body = Some body.
+Proof. Admitted.
+
+Lemma forward_assignments_body_writes body body' :
+  forward_assignments_body body = inr body' ->
+  module_body_writes body' = module_body_writes body.
+Proof.
+  intros H.
+  funelim (forward_assignments_body body);
+    rewrite <- Heqcall in *; clear Heqcall; monad_inv;
+    [reflexivity|].
+  simp module_body_writes module_item_writes statement_writes expr_reads.
+  rewrite H by auto.
+  rewrite apply_substitution_writes.
+  reflexivity.
+Qed. 
+
+Lemma forward_assignments_body_sorted body body' :
+  NoDup (module_body_writes body) ->
+  module_items_sorted body ->
+  forward_assignments_body body = inr body' ->
+  module_items_sorted body'.
+Proof.
+  intros Hnodup Hsorted Hforward.
+  funelim (forward_assignments_body body);
+    rewrite <- Heqcall in *; clear Heqcall; monad_inv;
+    [assumption|].
+  inv Hsorted.
+  autorewrite with
+    expr_reads module_item_reads statement_reads
+    module_body_writes module_item_writes statement_writes
+    in *.
+  disjoint_saturate.
+  constructor.
+  - autorewrite with
+      expr_reads module_item_reads statement_reads
+      module_body_writes module_item_writes statement_writes
+      in *.
+      simpl.
+      erewrite forward_assignments_body_writes; eauto.
+      rewrite apply_substitution_writes.
+      constructor; crush.
+  - eapply H.
+    + rewrite apply_substitution_writes. assumption.
+    + apply apply_substitution_sorted; eauto.
+    + reflexivity.
+Qed.
+
+Lemma forward_assignments_correct regs v1 v2 :
+  forward_assignments v1 = inr v2 ->
+  run_vmodule v1 regs = run_vmodule v2 regs.
+Proof.
+  intros.
+  unfold forward_assignments, run_vmodule, opt_to_sum in *.
+  monad_inv. simpl in *.
+  rewrite ! sort_module_items_idempotent
+    by eauto using forward_assignments_body_sorted.
+  replace (mk_initial_state
+     {| modName := modName v1; modVariableDecls := modVariableDecls v1; modBody := l |} regs)
+     with (mk_initial_state v1 regs) by now apply initial_state_same.
+  symmetry.
+  now apply forward_assignments_body_correct.
+Qed.
+
+Lemma equal_exact_equivalence v1 v2 :
+  module_inputs v1 = module_inputs v2 ->
+  module_outputs v1 = module_outputs v2 ->
+  (forall regs, run_vmodule v1 regs = run_vmodule v2 regs) ->
+  v1 ~~~ v2.
+Proof.
+  intros Hinputs Houtputs Hmatch.
+  constructor; try eassumption; expect 1.
+  intros regs.
+  unfold "⇓".
+  rewrite Hinputs, Houtputs, Hmatch.
+  reflexivity.
+Qed.
+
+Lemma assignment_forwarding_exact_equivalence v1 v2 :
+  AssignmentForwarding.forward_assignments v1 = inr v2 ->
+  v1 ~~~ v2.
+Proof.
+  intros H.
+  apply equal_exact_equivalence.
+  - apply module_inputs_same.
+    unfold forward_assignments in *. monad_inv. reflexivity.
+  - apply module_outputs_same.
+    unfold forward_assignments in *. monad_inv. reflexivity.
+  - intros.
+    apply forward_assignments_correct.
+    assumption.
+Qed.
+
+Print Assumptions assignment_forwarding_exact_equivalence.
